# Writing Math Proofs

Dr. Daniel Slilaty

MM232 2:30-3:20 MWF & 1:00-1:50 TR

## Chapter 1: Propositional Logic

Proposition (or Statement): A sentence that has a definite truth value. (T/F)

Example:

1. "4 is even" (T)
2. "9 is a prime number" (F)
3. "Mark is a pilot" (T | F depending on who Mark is.)

Non-Example:

1. "Mark is tall" (Subjective, no definite T/F. "tall" is not clearly defined)
2. "Do you like chocolate?" (Question)
3. "Barnie horse" (Not a sentence)

Propositions may be put together into larger propositions using logical connectors.

### 1 Conjunction $\wedge$

Given propositions $A$ and $B$, $A \wedge B$ is a proposition whose truth value is given in the following table.

| $A$ | $B$ | $A  \wedge B$ |
| --- | --- | :-----------: |
| T   | T   |       T       |
| T   | F   |       F       |
| F   | T   |       F       |
| F   | F   |       F       |

$A \wedge B$ can be written in English as

1. A and B
2. A but B
3. A however B
4. A furthermore B
5. A. B.

Conjunction can also connect 3 or more propositions into one proposition.

$$A_{1} \wedge A_{2} \wedge A_{3}\wedge ... \wedge A_{n} $$

is true if each $A_{i}$ is true itself. That is, if any one $A_{i}$ is false, the conjunction $A*{1} \wedge A*{2} \wedge A*{3} ... \wedge A*{n} $ is false.

### 2 Disjunction $\vee$

Given propositions $A$ and $B$, $A \vee B$ is a proposition whose truth value is given in the following table.

| $A$ | $B$ | $A  \vee B$ |
| --- | --- | :---------: |
| T   | T   |      T      |
| T   | F   |      T      |
| F   | T   |      T      |
| F   | F   |      F      |

$A \vee B$ can be written in English as

1. A or B (Inclusive OR)
2. A or else B
3. Either A or B
4. If not A, then B

Disjunction can also connect 3 or more propositions into one proposition.

$$A_{1} \vee A_{2} \vee A_{3} \vee ... \vee A_{n} $$

is true if at least one $A_{i}$ is true. That is, if any one $A_{i}$ is true, the conjunction $A*{1} \vee A*{2} \vee A*{3} ... \vee A*{n} $ is true.

### 3 Implication $\implies$

Given propositions $A$ (Hypothesis) and $B$ (Conclusion), $A \implies B$ is a proposition whose truth value is given in the following table.

| $A$ | $B$ | $A  \implies B$ |
| --- | --- | :-------------: |
| T   | T   |        T        |
| T   | F   |        F        |
| F   | T   |        T        |
| F   | F   |        T        |

When the hypothesis is false, the implication is always true. The conclusion is irrelevant when the hypothesis is false.

$A \implies B$ can be written in English as

1. A implies B
2. If A, then B
3. B wehn A
4. B if A
5. B is necessary for A
6. A is sufficient for B

X is sufficient for Y = $X \implies Y$

These all descrbe a containment relationship. Instances where A is true are contained in instances when B is true.

### 4 Logical Equivalence $\iff$

Given propositions $A$ and $B$ , $A \iff B$ is a proposition whose truth value is given in the following table.

| $A$ | $B$ | $A  \iff B$ |
| --- | --- | :---------: |
| T   | T   |      T      |
| T   | F   |      F      |
| F   | T   |      F      |
| F   | F   |      T      |

### 5 Negation $ \neg $

Given propositions $A$, $ \neg A $ is a proposition whose truth value is given in the following table.

| $A$ | $ \neg A$ |
| --- | --------- |
| T   | F         |
| F   | T         |

## Boolean Arithmetic

_**Operator Precedence**_

1. $ \neg $
2. $ \wedge , \vee $ neither have precedence over the other
3. $ \implies $
4. $ \iff $

- $A \wedge B \implies C \ (1)$ means $(A \wedge B) \implies C \ (2)$, not $A \wedge (B \implies C) \ (3)$

To produce $(2)$, the parenthesis are necessary. To produces $(3)$, the parenthesis are not necessary.

- $A \wedge B \vee C$ is ambigious and has no meaning. You must write $(A \wedge B) \vee C$ or $A \wedge (B \vee C)$

## Truth Tables

Given a compound propositional logic statement, a truth table shows the truth value of htat statement for all possible truth combinations of the bare propositions from which it is composed.

$$ \rule{4cm}{0.1pt} $$
$$A \wedge (B \implies C)$$

$$ \rule{6cm}{0.1pt} $$

| $A$ | $B$ | $C$ | $B \implies C$ | $A \wedge (B \implies C)$ |
| :-: | :-: | :-: | :------------: | :-----------------------: |
|  T  |  T  |  T  |       T        |             T             |
|  T  |  T  |  F  |       F        |             F             |
|  T  |  F  |  T  |       T        |             T             |
|  T  |  F  |  F  |       T        |             T             |
|  F  |  T  |  T  |       T        |             F             |
|  F  |  T  |  F  |       F        |             F             |
|  F  |  F  |  T  |       T        |             F             |
|  F  |  F  |  F  |       T        |             F             |

### Laws of Logic

![Alt text](./image-7.png)
![Alt text](./image-8.png)

### Tautologies

![Alt text](image-9.png)
$ \rule{ 12cm }{0.1pt} $

$ \rule{ 12cm }{0.1pt} $

Tautology: A logic statement which is always true is a tautology.

Example:

$$A \wedge B \implies C \iff A \implies (B \implies C)$$

Implication -> DeMorgan's Law -> Associativity -> Implication -> Implication

$$A \wedge (A \implies B) \implies B \iff 1$$

Implication -> Implication -> Distribution -> Complement -> Identity -> Demorgan -> Associativity -> Complement -> Annhilation (Null)

## English to Predicate Logic

- H = "The horse is fresh"

- A = "Armor is strong"

- K = "The knight will win"

- O = "The opponent cheated"

1. If the horse is fresh and the armor is strong then the knight will win

   - $H \wedge A \implies K$

2. The knight will win only if the horse is fresh.

   - $H \implies K$ is wrong. Use containment to find. Try with $K \subset H$ or $H \subset K$ and take a point outside the subset but inside the set. The one that contradicts the original statement is wrong.

3. The knight will win if the horse is fresh.

   - $H \implies K$

4. The knight will win iff the horse is fresh.

   - $K \iff H$

5. It suffices to say that the knight loses only when the opponent cheated.

   - $K' \implies O$ or $O \implies K'$ ?

   - $K' \subset O$ - A point says: The knight won and the opponent cheated.

   - $O \subset K'$ - A point says: The knight lost and the opponent followed the rules. CONTRADICTS the original statement, therefore is wrong.

6. The knight lost, the armor was strong, and the opponent cheated or the horse was tired.

   - $K' \wedge A \wedge (O \vee H')$

7. The knight lost, the armor was strong and the opponent cheated, or the horse was tired.

   - $K' \wedge (A \wedge O) \vee H'$

## Negating English

1. Translate English -> Propos. Logic
2. Negate the Propos. Logic
3. Translate Propos. Logic -> English

## Important tautolgy

$$(A \implies B)' \equiv A \wedge B'$$

Examples:

1. If the restaurant is good, then the prices are high.

$G \implies H$ -> $(G \implies H)'$ -> $(G' \vee H)'$ -> $(G' \vee H)'$ -> $(G \wedge H')$ -> "The restaurant is good but the prices are reasonable."

2. If the restaurant is good and the service is fast, then the prices are high.

$G \wedge F \implies H \equiv (G \wedge F \implies H)' \equiv^{negated \ implication} (G \wedge F) \wedge H' \equiv G \wedge F \wedge H'$

The restaurant is good, the service is fast, but the prices are reasonable.
`and` or `;however,` work.

3. Either the food is bad and the service is bad or the restaurant will not profit.

$(F \wedge S) \vee P' \equiv ((F \wedge S) \vee P')' \equiv ((F \wedge S)' \wedge P) \equiv ((F' \vee S') \wedge P) $

The restaurant will profit even though the food or service is acceptable.

4. The resataurant is good iff the food is good.

$R \iff F \equiv ((R \implies F) \wedge (F \implies R))' \equiv (R \implies F)' \vee (F \implies R)' \equiv (R \wedge F') \vee (F \wedge R')$

Either the restaurant is good and the food is not, or the food is good and the restaurant is not.

Either the restaurant is good or the food is good, but not both. (XOR $\oplus $)

## XOR $\oplus$

| $A$ | $B$ | $A \oplus B$ |
| :-: | :-: | :----------: |
|  T  |  T  |      F       |
|  T  |  F  |      T       |
|  F  |  T  |      T       |
|  F  |  F  |      F       |

## More Examples for Translating E -> Propositional logic

B = "Bears are happy"

F = "Fish are plentiful"

S = "There is heavy snow"

a. Plentiful fish is sufficient for bears to be happy.

- $F \implies B$

b. Bears are happy ONLY IF there's plentiful fish.

A happy bear implies the existence of plentiful of fish around.

- $B \implies F$

c. Unhappy bears means fish are not plentiful and also there is heavy snow.

- $B' \implies F' \wedge S$

d. Unhappy bears is necessary for heavy snow.

- $?$

e. The fish are not plentiful **IF** the snow is heavy.

The if thing is the hypothesis. But if it's "only if" then it's the conclusion.

- $S \implies F'$

f. The fish are not plentiful **ONLY IF** the snow is heavy.

- $F' \implies S$

g. The fish are not plentiful **IF AND ONLY IF** the snow is heavy.

- $F' \iff S$

## Predicate Logic

Example:

$E(x)$ = "x is even"

$E(4)$ is T

$E(3)$ is F

$$\rule{4cm}{0.1pt}$$

$S(x,y)$ = "x+y=10"

$S(3,7)$ is true

$S(7,3)$ is true

$S(1,1)$ is false

$$\rule{4cm}{0.1pt}$$

P(x,y) = "x is the parent of y"

P(Jane, Bobby) is true when Jane is the parent of Bobby. In which case, P(Bobby, Jane) is false.

Other than just plugging in values for the variables of predicates, we can also do what is known as quantifying variables over a domain.

A domain D is a set of values which may be plugged into the variables of a predicate.

### Universal quantification ($\forall x$)

$\forall{x} P(x)$

Means

"For all x, P(x) is true."

"For each x, P(x) is true."

"Every x makes P(x) true."

Formerly, $\forall{x} P(x)$ is true over domain $D$ when for any $d \in D$, $P(d)$ is true.

### Existential Quantification ($\exists x$)

$\exists{x} P(x)$

Means

"There is some x which makes P(x) true."

"Some x makes P(x) true."

Formerly, $\exists{x} P(x)$ is true over domain $D$ when there is at least one $d \in D$ for which $P(d)$ is true.

### Examples

Consider the domains:

$D_{1} = \{1,2,3,4,5,...\}$

$D_{2} = \{...,-1,0,1,2,3,...\}$

$D_{3} = \{0,1,2,3,...\}$

1. $(\forall x)(x > 0)$

$D_{1}$ -> True

$D_{2}$ -> False

$D_{3}$ -> False

2. $(\forall x)(x \ge 0)$

$D_{1}$ -> True

$D_{2}$ -> False

$D_{3}$ -> True

3. $(\exists x)(x \le 0)$

$D_{1}$ -> False

$D_{2}$ -> True

$D_{3}$ -> True

4. $(\exists x)(x \gt 0)$

$D_{1}$ -> True

$D_{2}$ -> True

$D_{3}$ -> True

### Stacking Quantifiers

1. $(\forall x)(\forall y) P(x,y)$ means the same as $(\forall y)(\forall x) P(x,y)$

2. $(\exists x)(\exists y) P(x,y)$ means the same as $(\exists y)(\exists x) P(x,y)$

3. $(\forall x)(\exists y) P(x,y)$ means given a fixed singular element $x$ in the domain, $\exists y  P(x,y)$ is true,. That is, for any fixed x in the domain, there is a y which goes along with x to make $P(x,y)$ true.

4. $(\exists y) (\forall x) P(x,y)$ means there is a singular universal $y$ in the domain which satisfies $(\forall x) P(x,y)$. There is a universal $y$ that goes along with every $x$ to make $P(x,y)$ true.

| Example                         | $\{..,-2,-1,0,1,2,...\}$ |  $\{1,2,3,4,5,..\}$   | $\{0,1,2,3,..\}$ |
| :------------------------------ | :----------------------: | :-------------------: | :--------------: |
| $(\forall x)(\exists y)(x+y=0)$ |            T             |           F           |        F         |
| $(\exists y)(\forall x)(x+y=0)$ |            F             |           F           |        F         |
| $(\forall x)(\exists y)(xy=0)$  |            T             | F ($0 \notin$ domain) |        T         |
| $(\exists y)(\forall x)(xy=0)$  |            T             | F ($0 \notin$ domain) |        T         |

Question: Is there a domain over which $(\exists y)(\forall x)(x+y=0)$ is true?

Yes, $D=\{0\}$

## Scope of a Quantifier

$(\forall x)(P(x) \implies Q(x))$

The $(\forall x)$ quantifier applies to the predicate statement immediately to its right and no further.

$(\forall x)P(x) \implies (\exists y) Q(y)$

since the scope of the two quantifiers don't overlap, we actually could use the letter x twice. Like:

$(\forall x)P(x) \implies (\exists x) Q(x)$

Meaning: If everything in the domain satisfies $P(x)$ then something in the domain satisfies $Q(x)$

## Translating English to Predicate Logic Statememnts

Usually when doing this exercise, we assume the domain is the entire universe, both real and imagined.

Two principles are used here:

1. When universally quantifying a subset of your domain which is identified by $P(x)$, then we write $(\forall x)(P(x) \implies ...)$
   - We never write $(\forall x)(P(x) \wedge ...)$ this statement is automatically false, despite whatever $P(x)$ might mean.

Example:

$P(x)$ = "x is a potato"

$B(x)$ = "x is brown"

"All potatoes are brown" is $(\forall x)(P(x) \implies B(x))$, it is NOT $(\forall x)(B(x))$ means "everything is brown."

2. When existentially quantifying some subset of your demain which is identified by $P(x)$, then we write $(\exists x)(P(x) \wedge ...)$
   - We never write $(\exists x)(P(x) \implies ...)$ This statement is automatically true despite whatever $P(x)$ might mean.

Example:

$P(x)$ = "x is a potato"

$B(x)$ = "x is brown"

"Some potatoes are brown." is $(\exists x)(P(x) \wedge B(x))$

NOT $(\exists x) B(x)$ which means something in the universe is brown.

$$\rule{4cm}{0.1pt}$$

Examples:

$P(x)$ = "x is a pony"

$G(x)$ = "x eats grass"

$R(x)$ = "x runs fast"

1. "All ponies eat grass"

- $(\forall x)(P(x) \implies G(x))$

2. "Only ponies eat grass"

- $(\forall x)(G(x) \implies P(x))$

- or $(\forall x)(P'(x) \implies G'(x))$

The statement can be restated as "If it eats grass, then it 's a pony." or "If it's not a pony, then it doesn't eat grass" (Contrapositive)

3. "All grass-eating ponies run fast"

Notice that

$P(x)$ = "x is a pony"

$G(x)$ = "x eats grass"

$G(x) \wedge P(x)$ - "x is a pony that eats grass."

$(\forall x)(G(x) \wedge P(x) \implies R(x))$

- $\forall x$ dont use $\wedge$

- $\exists x$ dont use $\implies$

4. "No ponies run fast"

- $(\forall x)(P(x) \implies R'(x))$

5. "Some ponies run fast"

- $(\exists x)(P(x) \wedge R(x))$

6. "Not all ponies eat grass" or "Some ponies don't eat grass"

- $(\exists x)(P(x) \wedge G'(x))$

### Multiple Quantification

$B(x)$ = "x is a bee"

$F(x)$ = "x is a flower"

$L(x,y)$ = "x likes y"

$D$ = Whole universe and everything in it

1. "Some bees like all flowers"

- $(\exists x) (B(x) \wedge (\forall y)(F(y) \implies L(x,y)))$

This is equivalent to

- $(\exists x) (\forall y) (B(x) \wedge (F(y) \implies L(x,y)))$

2. "All bees like some flowers"

- $(\forall x) (B(x) \implies (\exists y)(F(y) \wedge L(x,y)))$

3. "All bees like all flowers"

- $(\forall x)(B(x) \implies (\forall y)(F(y) \implies L(x,y)))$

Via exportation tautology: $P \implies (Q \implies R) \equiv P \wedge Q \implies R$

- $(\forall x) (\forall y)(B(x) \wedge F(y) \implies L(x,y))$

4. "Some bees like some flowers"

- $(\exists x)(\exists y)(B(x) \wedge F(y) \wedge L(x,y))$

5. "Some bees don't like flowers"

- $(\exists x)(B(x) \wedge (\forall y)(F(y) \implies L'(x,y)))$

6. "No bees like all flowers."

"All bees don't like all flowers"

"Every bee has some flower it doesn't like"

- $(\forall x)(B(x) \implies (\forall y)(F(y) \implies L'(x,y)))$

Via exportation tautology: $P \implies (Q \implies R) \equiv P \wedge Q \implies R$

- $(\forall x)(B(x) \implies (\exists y)(F(y) \wedge L'(x,y)))$

## Interpretations

Given an abstract predicate logic statement, an "interpretation" consists of two things:

1. Domain
2. Meanings for the predicates

... Notes Here ...

### Example 2

$(\forall x)(H(x) \implies M(x)) \wedge (\exists x)(H(x)) \implies (\forall x)M(x)$

Interpretation where the statement is false

$D=\{1,2,3,4,5,...\}$

Interpretation that

- M(x) = "x is even"

- H(x) = "x is a multiple of 4"

x = 2 makes the statement false.

## More examples of English to Predicate Logic

$B(x)$ = "x is a bee"

$F(x)$ = "x is a flower"

$L(x,y)$ = "x likes y"

$N(x)$ = "x smells nice"

### Remember

- All bees ... $\equiv$ $(\forall x)(B(x) \implies ...)$

- Some bees ... $\equiv$ $(\exists x)(B(x) \wedge ...)$

## Basics of Naive Set Theory

A set is a collection of objects called elements presented in no particular order and always perhaps with some repetition in the presentation.

$x \in A$ is a predicate saying $x$ is an element of set A

$x \notin A$ is a predicate saying $x$ is NOT an element of set A

Anything can be an element of a set, including other sets.

One way to describe a set is between braces $\{\}$ with elements delimited by commas $,$

- ${1,5,-3,2,\triangle, \pi}$ is a set of 6 elements.

- This is the same set ${1,-3,5,2,\triangle, \pi}$ because the order does not matter.

- This is also the same set ${1,1,1,1,-3,5,2,\triangle, \pi}$ because an element is either in or not in a set. It's never in a set multiple times.

- Here is a set with three elements. A set can be an element of a set. $\{1,2,\{5,7,9\}\}$

### Set Builder Notation

$$\{ x\ |\ P(x) \}$$

The set of all elements $x$ such that $P(x)$ is true.

#### Example

The set of natural numbers is

$$\N = \{0,1,2,3,4,...\}$$

The set of integers ("zahlen" in German) is

$$\Z = \{x, -x\ | x \in \N\}$$

The set of rational numbers is

$$ Q = \{\frac{a}{b}\ |\ a \in \Z \wedge b \in \Z \wedge b \neq 0\}$$

### Russel's Paradox

We have said that sets can be elements of other sets. so now:

let $X = \{ B \ |\ B \in B\}$ and $Y = \{ B \ |\ B \notin B\}$

If $Y \in X$ then $Y \in Y$ but by definition but being an element of $Y$ implies $Y \notin Y$ by its own definition.

If $Y \in Y$ then by definion, $Y \notin Y$ so $Y$ can belong to neither $X$ nor $Y$ but the statement $Y \in Y$ should be true or false.

### Subsets

When we say $A \subseteq B$ (read as a $A$ is a subset of $B$)
when $$(\forall x)(x \in A \implies x \in B)$$ is true.

#### Example

For any set $A$, $A \subseteq A$ is always true.

$\phi$ denotes the empty set. It is a set containing no elements that is $x \in \phi$ is false for all x. Therefore

$(\forall x)(x \in \phi \implies x \in A)$

$\phi \subseteq A$ is true for any set A.

### Power Set

$$\wp (A) = \{B\ |\ B \subseteq A\}$$

Given a set $A= \{1,2,3\}$, the power set of $A$ is every combination of elements. Its elements are
$$\wp (A) = \{\phi,\{1\},\{2\},\{3\},\{1,2\}, \{2,3\},\{1,3\}, \{1,2,3\}\}$$

$$|\wp (A)| = 2^{|A|}$$

Because a subset $B \subseteq A$ is constructed by considering each element $x \in A$ and choosing either $x \in B$ or $x \in B$. This is 2 choices for the $|A|$ elements. Therefore, there are $C_{2}^{|A|}$ possible outcomes for $B$.

## Laws of Set Theory

$$ A - B = A \cap B'$$

![Alt text](image-10.png)

**Disjoint Sets:** Two sets are disjoint if they have no elements in common. That is, $A$ and $B$ are disjoint if $A \cap B = \phi$.

**Pairwise Disjoint:** A collection of sets $A_{1}, A_{2}, ..., A{n}$ are pairwise disjoin when $A_{i} \cap A_{j} = \phi$ for all $i \neq j$

**Compliment of a Set:** $$A' = U - A$$
$$A' = \{x\ |\ x \notin A\}$$

**Symmetric Difference:**$(\oplus\ or\ \triangle)$ Let $A$ and $B$ be sets. $A \oplus B = (A \cup B) - (A \cap B)$ i.e. the elements that are in A and in B but not both. (XOR)

$A\ \triangle\ B = A$

$A \triangle B = \{x|(x\in A \vee x \in B) \wedge x \notin A \cap B\} =_{definition\ of\ complement} = ....$

**Order of a Set (Cardinality):** Number of elements in a set.

**Set subtraction:** $A-B$ means elements in $A$ but not in $B$.
$$A-B = \{x\ |\ x \in A \wedge x \notin B\} = \{x\ |\ x \in A \wedge x \in B'\} =  A \cap B'$$

### Examples

a. Let's prove that $A-B = A-(A \cap B)$

$A-(A\cap B) =_{set\ subtraction} A \cap (A \cap B)' =_{DeMorgan} A \cap (A' \cup B') =_{distribution} (A \cap A') \cup (A \cap B') =_{complement} \phi \cup (A \cap B') =_{identity} (A \cap B') =_{set\ subtraction} A - B$

b. $(A \cup B) - (A \cap B) = (A-B) \cup (B-A)$

$(A \cup B) - (A \cap B) =_{set\ subtraction} = (A \cup B) \cap (A \cup B)' =_{DeMorgan} (A \cup B) \cap (A' \cup B') =_{distribution\ x3} (A \cap A') \cup (A \cap B') \cup (B \cap A') \cup (B \cap B') =_{complement\ x2} = \phi \cup (A \cap B') \cup (B \cap A') \cup \phi =_{identity\ x2} ...$

## Missed Set Equality Proof 2/6

Set proofs start out with: Let $x \in A$ ...

### Example

Prove that $A \cap (A \cup B) = A$.

First prove $A \cap (A \cup B) \subseteq A$. Let $x \in A \cap (A \cup B)$. By the definition of intersection $x \in A$.

Now prove $A \subseteq A \cap (A \cup B)$. Let $x \in A$. By definiton of union $x \in A \cup B$. Therefore, by definition of intersection, $x \in A \cap (A \cup B)$ $\blacksquare$

$$\rule{8cm}{0.1pt}$$

Can we also prove that $A \cap (A \cup B) = A$ using basic set identities?

identity, distribution, annihilation, identity

### Try at home

Prove that $A \cup (A \cap B)$ using both methods.

## Proving Implications

P, Q are predicate statements, not sets.

$$P \implies Q$$

1. **Direct proof:**. Assume $P$ is true. Show $Q$ must be true as well.

2. **Contrapositive:** Assume $Q'$ is true. Show that $P'$ is true as well.

3. **Proof by Contradiction:** Assume $P$ is true and $Q$ is false. Conclude a contradiction.

$$C \subseteq A \cap B \iff (C \subseteq A) \wedge (C \subseteq B)$$

Prove it using a chain of logical equivalences... Check 2/8 Notes.

### Example

If $A \cap C \subseteq B$ and $B \cap C \subseteq A$, then $A \cap C = B \cap C$

#### Direct Proof

Assume $A \cap C \subseteq B$ and $B \cap C \subseteq A$. Show that conclusion is subset of eachother. See notes.

## Functions

Given a function $f:D\rightarrow R$, and a set $A \subseteq \R$ then the IMAGE of A is $$f(A) = \{f(x)\ |\ x \in A\} \subseteq \R$$

**Question** - Is the following statement True or False?

$$If\ z\in D\ and\ f(z)\in f(A),\ then\ z\in A$$

False. $f(\{1,2\}) = \{a\}$...

**Question**: Is the following true?

$$If\ f(A) \subseteq f(B),\ then\ A \subseteq B$$

False. A counterexample will need:

1. A function $f:D\rightarrow R$
2. $A,B \subseteq \R$ such that $A \not\subseteq B$
3. $f(A) \subseteq f(B)$

Consider $D = \{1,2\}$ and $R = \{1\}$.

$$f(\{1\}) = \{a\},\newline f(\{2\}) = \{a\}, \newline \{1\} \not\subseteq\{2\}\ but\ f(\{1\}) \subseteq f(\{2\})$$

**Question**: Is the following true for any function?

$f:D\rightarrow R$ and $A,B \subseteq D$.

"If $A \subseteq B$ then $f(A) \subseteq f(B)$"

Assume $A \subseteq B$. In order to prove $f(A) \subseteq f(B)$, consider $y \in f(A)$. By definition of image, there is a $x \in A$ such that $f(x) = y$. Because $A \subseteq B$, $x \in B$, also. By definition of image, $y = f(x) \in f(B)\ \blacksquare$

**Question**: Is the following true for any function?

$f:D\rightarrow R$ and $A,B \subseteq D$.

$f(A\cap B) \subseteq f(A) \cap f(B)$

Let $y \in f(A \cap B)$. By definition of image, there exists an $x \in A \cap B$. By definition of intersection, $x\in A \wedge x\in B$. By definition of image, $f(x) = y$. So, $y=f(x) \in f(A) \wedge y=f(x) \in f(b)$. Therefore, $y\in f(A) \cap f(B).\ \blacksquare$

**The other way around is NOT a subset, though.**

**Question**: Is the following true for any function?

$f:D\rightarrow R$ and $A,B \subseteq D$.

### $f(A) \cup f(B) = f(A \cup B)$

$f(A) \cup f(B) \subseteq f(A \cup B)$

Let $y \in  f(A) \cup f(B)$. By definitionof union, $y \in f(A)$ or $y \in f(B)$. Without loss of generality, we may assume $y \in f(A).$ By definition of image, there is $x \in A$ such that $f(x) = y$. By definition of union, $x \in A \vee x\in B$. By definition of image, $y=f(x) \in f(A \cup B)\ \blacksquare$

$f(A \cup B) \subseteq  f(A) \cup f(B)$

Let $y \in  f(A \cup B)$. By definitionof image, there is $x \in A \cup B$ such that $y=f(x)$. By definition of union, $x\in A$ or $x \in B$. Without loss of generality, we may assume $x\in A$. Therefore, $y=f(x)\in f(A)$. Therefore, by definitionof union, $y\in f(A \cup B)$

$$\rule{6cm}{0.1pt}$$
$$f(\phi) = \phi$$

## After Spring Break & Exam 1

### Preimages (NOT INVERSE)

Given a function $f: D \rightarrow R$ and $A \subseteq R$, the PREIMAGE of $A$ is:

$$f^{-1}(A) = \{x \in D\ |\ f(x) \in A\} \subseteq D$$

$$f^{-1}(\phi) = \phi$$

$f^{-1}(A)$

$f^{-1}(\{a\}) = \{x \in D\ |\ f(x) \in \{a\}\} = \{1,2,4\}$

Notice: The preimage of $f^{-1}(\{a\})=\{1,2,4\}$ whereas $f(\{1,2,4\}) = f(\{1\}) = f(\{1\}) = \{a\}$

**Preposition**: For any $f: D \rightarrow R$ and $A \subseteq R$, $x\in f^{-1}(A)$ if and only if $f(x) \in A$

**Remark**: If $B \subseteq D$, then $x \in B \implies f(x) \in f(B)$ but $f(x) \in f(B)$ does not imply $x\in B$

The proof of this statement is:

1. $x\in f^{-1}(A) \implies f(x) \in A$
2. $f(x) \in A \implies x\in f^{-1}(A)$

(1) Suppose that $x\in f^{-1}(A)$. By definition of preimage, $f(x) \in A$, as required.

(2) Suppose $f(x) \in A$. By definition of preimage, $x \in f^{-1}(A)$, as required.

**Better Proof:** By definition of preimage. $\blacksquare$

**Preposition:** For any $f: D \rightarrow R$ and $A \subseteq R$,

$$f^{-1}(A) \cap f^{-1}(B) = f^{-1}(A \cap B)$$

Proof:

$$f^{-1}(A) \cap f^{-1}(B) \subseteq f^{-1}(A \cap B)$$

Let $x \in f^{-1}(A) \cap f^{-1}(B)$. By def of intersection, $x \in f^{-1}(A)\wedge x \in f^{-1}(B)$. By definition of preimage, $f(x) \in A$ and $f(x) \in B$. Therefore, $f(x) \in A \cap B$. By def of preimage $x \in f^{-1}(A\cap B)$.

$$f^{-1}(A \cap B) \subseteq f^{-1}(A) \cap f^{-1}(B)$$

Let $x \in f^{-1}(A \cap B)$. By def of preimage, $f(x) \in A \cap B$. So, $f(x) \in A \wedge f(x) \in B$. So $x \in f^{-1}(A) \wedge x\in f^{-1}(B).$ So $x\in f^{-1}(A) \cap f^{-1}(B)$ $\blacksquare$

$$\rule{6cm}{0.1pt}$$

A better proof:

$x\in f^{-1}(A) \cap f^{-1}(B)$ iff (def of intersection)

$x\in f^{-1}(A) \wedge x\in  f^{-1}(B)$ iff (def of preimage)

$f(x) \in A \wedge f(x) \in B$ iff (def intersection)

$f(x) \in A \cap B$ iff (def of preimage) $x \in f^{-1}(A\cap B)\ \blacksquare$

### Preimages examples

Let $f: \Z \times \Z \rightarrow \N$ defined by $f((a,b)) = a^2 + b^2$

$f^{-1}(\{0\}) = \{(0,0)\}$

$f^{-1}(\{1\}) = \{(-1,0),(0,-1),(1,0),(0,1)\}$

$f^{-1}(\{0,1\}) = \{(-1,0),(0,-1),(1,0),(0,1),(0,0)\}$

$$f^{-1}(A)...$$

$f^{-1}({25}) = ...$

Is there some nice familiar geometric objects containing $f^{-1}(\{0,1,25\})$?

Answer: Circles of radius 0, 1, and 5.

## Properties of Functions

### Injective (One-to-one)

A function $f: D\rightarrow R$ is called injective when for all $a,b \in D$, $$f(a) = f(b) \implies a = b$$

Equivalently, for all $a,b \in D$, $a \neq b \implies f(a) \neq f(b)$

In terms of bubble diagrams, an element of R having to in-arrows means the function is not injective.

$$\rule{6cm}{0.1pt}$$

Consider the function $f: \R - \{4\} \rightarrow \R $ defined by $$f(x) = \frac{3x+1}{x-4}$$

Prove that $f$ is injective/one-to-one.

Suppose that $f(a) = f(b)$. In other words, $$\frac{3a+1}{a-4} = \frac{3b+1}{b-4} \newline ...\ solve\ ...\newline a = b$$

**Example**

A function $f: D \rightarrow \R$ where $D \subseteq R$ is injective if and only if the graph $y=f(x)$ satisfies the horizontal line test.

## More Examples of Image and Preimage

**Proposition** If $f:D\rightarrow R$ is a function and $A \subseteq D$ then $A \subseteq f^{-1}(f(A))$

**Proof**: Assume If $f:D\rightarrow R$ is a function and $A \subseteq D$ is true. Let $x \in A$. By def of image, $f(x) \in f(A)$. By def of preimage, $x \in f(f^{-1}(A))$

**Example** Show that $f^{-1}(f(A)) \subseteq A$

**Proposition** If $f:D\rightarrow R$ is a function and $B \subseteq R$ then $f^{-1}(f(B)) \subseteq B$

**Proof**:

### $f(f^{-1}(B))\subseteq B$

Let $y \in f(f^{-1}(B))$. By definition of image, $y=f(x)$ for some $x \in f^{-1}(B)$. By definition of preimage, $f(x) \in B$

### $B \subseteq f^{-1}(f(B))$

Let $y \in B$.

## Cont. Function Properties

**Injective**: One-to-one.

**Surjective**: Onto.

**Bijective**: Injective & Onto.

### Surjective

A function $f: D\rightarrow R$ is called surjective when for all $y \in R$, there is $x \in D$ such that $f(x) = y$.

Equivalently, if $B \subseteq R$ and $B\neq\phi$, then $f^{-1}(B) \neq \phi$

**Example**

$$f:(\R - \{4\}) \rightarrow (\R - \{3\})$$

$f(x) = \frac{3x-1}{x-4}$

We need to find a real number $x$ such that $f(x) = y$

$y(x-4) = 3x+1$

$xy-4y = 3x+1$

$xy-3x = 1+4y$

$x(y-3) = 1+4y$

$x = \frac{1+4y}{y-3}$

Which is a real number because $y \neq 3$.

### Bijection

When a function $f:D\rightarrow R$ is both injective and surjective, we call $f$ a bijection.

**Proposition** If $f: D \rightarrow R$ is surjective, and $B \subseteq R$ then $$f(f^{-1}(B)) = B$$

**Proof**:

### $f(f^{-1}(B))\subseteq B$

Let $y \in f(f^{-1}(B))$. By definition of image, $y=f(x)$ for some $x \in f^{-1}(B)$. By definition of preimage, $f(x) \in B$.

### $B \subseteq f^{-1}(f(B))$

Let $y \in B$. Because $f$ is surjective, there is an $x \in D$ such that $f(x) = y$. Therefore, by def of preimage $x \in f^{-1}(B)$. By definition of image, $y = f(x) \in f(f^{-1}(B)).\ \blacksquare$

## Inverse

Def: When $f: D \rightarrow R$ is a bijection, there is an inverse function $f^{-1}: R \rightarrow D$ where

$$f^{-1}(y) = x\ when\ f(x) =y$$

### Example

Given $f(x) = \frac{3x+1}{x-4}$ we can find $f^{-1}(x)$ by taking $y=\frac{3x+1}{x-4}$ and solving for $x$.

## Composition of Functions

Given two functions $f: A \rightarrow B$ and $g: C \rightarrow D$ define the composition $gf: A \rightarrow C$ as follows $$gf(a) = g(f(a))$$
The function $gf$ is called "g composed with f" or "g following f".

### Example

Consider the following six functions from subsets of $\R$ to subsets of $\R$

$$i(x) = x $$

$$b(x)= 1-x $$
$$c(x) = \frac{1}{x}$$
$$d(x) = \frac{1}{1-x}$$
$$e(x) = \frac{x}{x-1}$$
$$f(x) = \frac{x-1}{x}$$

- $be(x) = d(x) = \frac{1}{1-x}$

- $df(x) = i(x) = x$ this means that $d(x) = f^{-1}(x)$ or $f(x) = d^{-1}(x)$

- $f^2(x) = ff(x) = d(x) = \frac{1}{1-x}$

### Proposition

Consider $f: A \rightarrow B$ and $g: B \rightarrow C$. If $g$ and $f$ are both injective, then $gf$ is injective.

**Proof**: Assume $f,g$ are injective functions. To show that $gf$ is injective consider $p,q \in A$ such that $gf(p) = gf(q)$. Therefore $g(f(p)) = g(f(q))$ since $g$ is injective, $f(p) = f(q)$. Because $f$ is injective, $p = q\ \blacksquare$.

### Proposition

Consider $f: A \rightarrow B$ and $g: B \rightarrow C$.

If $gf$ is injectivem then $f$ is injective.

**Proof**: By way of contradiction, assume that $gf$ is injective, but $f$ is not injective. Because $f$ is not injective, there exists $p\neq q$ in $A$ such that $f(p) = f(q)$. Because $f(p) = f(q)$, when we apply $g$ we get $g(f(p)) = g(f(q))$. Thus, $gf(p) = gf(q)$. Because $gf$ is injective, we get $p=q$, which is a contradiction.

### Proposition

Consider $f: A \rightarrow B$ and $g: B \rightarrow C$. If $g$ and $f$ are both surjective, then $gf$ is surjective.

**Proof**: Assume $g,f$ are surjective. To show that $gf$ is surjective, consider an arbitrary $c \in C$.

### Proposition

Consider $f: A \rightarrow B$ and $g: B \rightarrow C$. If $gf$ is surjective, $g$ is surjective.

**Proof**: By way of contradiction, assume $gf$ is surjective but $g$ is not surjective. Therefore, there is $c \in C$ such that $g(b) \neq c$ for all $c \in C$. However, since $gf$ is surjective, there is some $a \in A$ such that $gf(a) = c$. Therefore $g(f(a)) = c$ where $f(a) \in B$ which is a contradiction.

### Summary of Proofs for Ch. 4

Consider $f: A \rightarrow B$ and $g: B \rightarrow C$.

1. If $f$ and $g$ are injective, then $gf$ is injective.
2. if $gf$ is injective, then $f$ is injective.
3. If $f$ and $g$ are surjective, then $gf$ is surjective.
4. If $gf$ is surjective, then $g$ is surjective.
5. **If $f$ and $g$ are bijective, then $gf$ is bijective.**
6. **If $gf$ is bijective, then $f$ is injective and $g$ is surjective.**

## Relations

Given a set $A$, a relation $R$ on $A$ is just a subset $R\subseteq A \times A$.

Notationally, however, relations are not written as ordered pairs of elements of $A$.

$$x \sim y\ ~when~\ (x,y)\in \R$$

### Examples

Given $\Z$ and $\le$ with its usual meaning gives a relation on $\Z$.

Given any set $A$ and a function $f:A\rightarrow A$, $f(x) = y$ means $x$ relates to $y$, which is a relation on $A$.

Given a set $A$ of propositional logic statements, say that preposition $P$ relates to proposition $Q$ when $P \implies Q$ is true. This is also a relation of $A$.

### Equivalence Relations

A relation $\sim~or~\equiv$ on set $A$ is an equivalence relation when $\sim$ satisfies the following three properties:

1. **Reflexive:** For all $x \in A$, $x \sim x$.
2. **Symmetric:** For all $x,y \in A$, $x \sim y$ implies $y \sim x$
3. **Transitive:** For all $x,y,z \in A$, $x\sim y$ and $y\sim z$ implies $x\sim z$

**Non-Example:** Consider the relation $\le$ with its usual meaning on $\Z$. This is not an equivalence relation because it's not symmetric.

### Example

Define $\equiv$ on $\Z$ by $x\equiv y$ when $x-y$ is even.

Let's prove it's an equiv. relation.

1. **Reflexivity**: Let $x \in \Z$. $x-x=0$, which is even. Thus, $x\equiv x$.
2. **Symmetric:** Let $x,y \in \Z$ such that $x\equiv y$. Since $x-y$ is even, then $y-x$ is also even even. $y-x = -(x-y)$ Thus, it is symmetric.
3. **Transitive:** Let $x,y,z \in \Z$ and $x\equiv y$ and $y\equiv z$. By definition of $\equiv$, that gives $x-y$ and $y-z$ are even. Which is true iff $\frac{x-y}{2}$ and $\frac{y-z}{2}$ are integers. Therefore $$\frac{x-y}{2} + \frac{y-z}{2} = \frac{x-z}{2}$$ Therefore, $x-z$ is even. Thus, $x\equiv z$.

### Practice

Define this relation $\equiv$ on $\Z$ by $x\equiv y$ when $x+y$ is even.

Prove that $\equiv$ is an equivalence relation.

Properties concerning addition and parity in $\Z$.

- For two integers $m,n \in \Z$:

  1. If $m$ and $n$ have the same parity, then $m+n$ is even.
  2. If $m$ and $n$ have different parity, then $m+n$ is odd.

1. **Reflexivity:** Let $x \in \Z$. $x+x=2x$, which is even. Thus, $x\equiv x$.
2. **Symmetric:** Let $x,y \in \Z$ such that $x\equiv y$. By definition of $\equiv$, $x+y$ is even. Therefore, $y+x=x+y$. Thus, $y\equiv x$
3. **Transitive:** Let $x,y,z \in \Z$ and $x\equiv y$ and $y\equiv z$. By definition of $\equiv$, that gives $x+y$ and $y+z$ are even. Thus, $x,y$ have the same parity. Also, $y,z$ have the same parity. Therefore, $x,z$ have the same parity, and thus $x+z$ is even. Thus, $x\equiv z.\ \blacksquare$

### Partitions

Let $A$ be any set. A Partition of $A$ is a collection $A_{1}, A_{2},...,A_{n}$ of non-empty, pairwise disjoint subsets of $A$ such that $A_{1} \cup A_{2} \cup ... \cup A_{n} = A$

That is

1. Each $A_{i} \ne \phi$.
2. For each $i\ne j$, $A_{i} \cap A_{j} = \phi$
3. $A_{1} \cup A_{2} \cup ... \cup A_{n} = A$

The subsets $A_{1}, A_{2},...,A_{n}$ are called the blocks of the partition.

### Example

Find all partitions of $\{1,2,3,4\}$

One-block partitions: $\{\{1,2,3,4\}\}$

Two-block partitions: $\{\{1,2,3\},\{4\}\}$ and $\{\{1,2,4\},\{3\}\}$ and $\{\{1,3,4\},\{2\}\}$ and $\{\{2,3,4\},\{1\}\}$ ... 2 - 2

Three-block partitions: $\{\{1\},\{2\},\{3,4\}\},\newline\{\{2\},\{3\},\{1,4\}\},\newline\{\{3\},\{4\},\{1,2\}\},\newline\{\{3\},\{1\},\{2,4\}\},\newline\{\{4\},\{2\},\{1,3\}\},\newline\{\{4\},\{1\},\{2,3\}\}$

So there are 15 partitions of $\{1,2,3,4\}$

### Example of Partition Relation

Let $A$ be any set and $B_{1}, B_{2},...,B_{n}$ be the blocks of a partition of $A$. Define a relation $\sim$ on $A$ by $x\sim y$ when $x,y \in A_{i}$. That is, $x,y$ are in the same block.

Prove that it's an equivalence relation.

1. Reflexive: Let $x\in A$. Certainly, $x$ is in the same block as itself, so $x \sim x$.
2. Symmetric: Let $x,y\in A$ such that $x\sim y$, that is $x,y \in B_{i}$. Since $x,y$ are in the same block, certainly $y,x$ are in the same block. Thus, $y \sim x$
3. Transitivity: Let $x,y,z \in A$ and $x\sim y$ and $y \sim z$. Since $x,y\in B_{i}$ and $y,z \in B_{j}$. However, $y$ is only in ONE block, so $i=j$. Therefore, $x,z$ are in the same block. So, $x\sim z$.

**Every equivalence relation is also a partition relation.**

### Example on Symmetric Difference $\oplus$

Given a set $X$, let $\wp (X)$ be the power set of $X$, that is $\wp (X) = \{A\ | A\  \subseteq X\}$ Define a relation $\equiv$ on $\wp (X)$ on when $|A\oplus B|$ is even.

$$O(X) = \{A \subseteq X\ |\ |A|\ is\ odd\}$$
$$E(X) = \{A \subseteq X\ |\ |A|\ is\ even\}$$

Now, let $A,B \in \wp(X)$, that is $A, B\subseteq X$.

Suppose $A,B \in E(X).$

$$|A \oplus B| = |(A-B) \cup (B-A)| = |A-B| + |B-A| (Because~there~is~no~overlap!) = \newline|A-(A\cap B)| + |B-(A\cap B)| = |A|-|A\cap B| + |B|-|A\cap B| = |A|+|B|-2|A\cap B|$$

which is even. Therefore, $A\equiv B$.

Suppose $A,B\in O(X).$

$$|A\oplus B| = |A| + |B| - 2|A\cap B|$$

which is even. Therefore, $A \equiv B$.

Suppose $A \in E(X)$ and $B \in O(X)$ then

$$|A\oplus B| = |A| + |B| - 2|A\cap B|$$

which is odd. Therefore, $A \not\equiv B$.

1. $A\oplus A = \phi$
2. $A \oplus B =  (A\cup B)-(A\cap B) = B \oplus A$
3. Transivity is long.

### Example

Consider the partition of $\Z$ into two blocks $E,O$:
$$E = \{n \in \Z\ |\ n\ is\ even\}$$
$$O = \{n \in \Z\ |\ n\ is\ odd\}$$

Recall that $x+y$ is even iff $x,y\in E$ or $x,y\in O$

Therefore the equivalence relation $x\equiv y$ when $x+y$ is even, is the partition relation given by $E$ and $O$.

Also, the parity of a number is unchanged under negation. Therefore the equivalence relation $x\equiv y$ when $x-y = x+(-y)$ is also given by the partition $E$ and $O$.

So the equivalence relations with different definitions are not different equivalence relations.

### Example

Let $\sim_{A}$ be an equivalence relation on a set $A$.

Let $\sim_{B}$ be an equivalence relation on a set $B$.

Define a relation $\sim$ on $A\times B$ by $(a_{1},b_{1})\sim (a_{2},b_{2})$ when $a_{1} \sim_{A} a_{2}$ and $b_{1} \sim_{B} b_{2}.$

Let's prove that $\sim$ is an equivalence relation on $A \times B$.

1. Reflexive: Let $(a,b) \in A \times B$. Because $\sim_{A}$ and $\sim_{B}$ are reflexive. By the definition of $\sim$, $(a,b) \sim (a,b)$.
2. Symmetric: Let $(a_{1},b_{1}), (a_{2},b_{2}) \in A \times B$ such that $(a_{1},b_{1}) \sim (a_{2},b_{2})$. By definition of $\sim$, $a_{1} \sim_{A} a_{2}$ and $b_{1} \sim_{B} b_{2}.$ Because $\sim_{A}$ and $\sim_{B}$ are both symmetric, $a_{2} \sim_{A} a_{1}$ and $b_{2} \sim_{B} b_{1}$. so $(a_{2},b_{2}) \sim (a_{1},b_{1})$
3. **Transitive check notes. TOO LONG!**

### Equivalence Classes

Let $\sim$ be an equivalence relation on a set $A$. For each $x \in A$, define its **equivalence class.**

$$[x] = \{~y\ |\ x \sim y~\}$$

**Remark** Saying $y \in [x]$ is equivalent to saying $x \sim y$ which is equivalent to saying $y \sim x$ because of symmetry.

**Proposition:** Let $\sim$ be an equivalence relation on $A$. The following are all true.

1. $x\in[x]$
2. $y \in [x]$ iff $[y]=[x]$
3. $y \not\in [x]$ iff $[y] \cap [x] = \phi$

**Proof of 1:** Because $\sim$ is reflexive, $x\sim x$. Therefore $x\in [x]$.

**Proof of 2:** Since $y \in [x]$, then $x \sim y$. Prove $$y\in [x] \implies [y]=[x]$$ and $$[y] = [x] \implies y\in [x]$$

#### $y\in [x] \implies [y]=[x]$

Assume $y\in [x]$. This means $x \sim y$ and $y \sim x$. In order to show that $[y] = [x]$ we must prove $[x] \subseteq [y]$ and $[y] \subseteq [x]$.

a. $[x] \subseteq [y]$: Let $z \in [x]$. This implies $x \sim z$ and $z \sim x$. Now because $x \sim y$, transitivity yields $z \sim y$. This implies $z \in [y].$

b. Let $[y] \subseteq [x]$: Analogous to the previous proof.

#### $[y] = [x] \implies y\in [x]$

Assume $[y] = [x]$. Since $y \in [y]=[x]$ we get $y \in [x]$.

**Proof of 3:** Double implication.

#### $(\rightarrow)$

Assume $y \in [x]$, that is $x \not\sim y$ and $y \not\sim x$.

By way of contradiction, assume that $[x] \cap [y] \neq \phi$ that means that there is an element $z\in [x] \cap [y]$ that is $z\in [x]$ and $z\in [y]$. This means that $x\sim z$ and $z \sim y$. Transitivity implies that $x \sim y$ which implies $y \in [x]$, a contradiction.

#### $(\leftarrow)$

Assume that $[x] \cap [y] = \phi$. Because $y \in [y]$ we now get that $y\not\in [x].~\blacksquare$

$$\rule{8cm}{0.1pt}$$

Thus two equivalence classes are either the same or disjoint with equality $[x]=[y]$ iff $x\sim y$ thus the equivalence classes partition $A$. Therefre equivalence relation $\sim$ is a partition relation.

So all equivalence relations and partition relations are the same thing.

### Example

Let $Z_{+} = \{1,2,3,4,...\}$ Define a relation $\sim$ on $Z_{+} \times Z_{+}$ by $(a,b) \sim (m,n)$ when $an=bm$.

Show it's equiv. relation:

**Reflexive:** Let $(a,b)\in Z_{+} \times Z_{+}$. Because $ab=ab$, we get $(a,b)\sim (a,b)$

**Symmetric:** Let $(a,b), (m,n) \in Z_{+} \times Z_{+}$. By definition we get $an=bm$ which implies that $mb=na$ which implies that $(m,n)\sim (a,b)$.

**Transitive:** Let $(a,b), (m,n), (x,y) \in Z_{+} \times Z_{+}$ and assume $(a,b) \sim (m,n)$ and $(m,n) \sim (x,y)$. By definition, $$an=bm~and~my=nx$$
Now, $n=\frac{my}{x}$ yields $$a\frac{my}{x}=bm$$ $$amy = bmx$$ $$ay = bx$$

Which means $(a,b) \sim (x,y)$

**Equivalence classes?**

Let $a,b$ have no common divisor. Now $[(a,b)] = \{(x,y)~|~ay=bx~\}=\{(x,y)~|~\frac{a}{b}=\frac{x}{y}\}$

Where $\frac{a}{b}$ positive rational number in simplest form. Therefore $\frac{x}{y}=\frac{da}{db}$ where $d$ is a common divisor of $x$ and $y$.

$$[(a,b)] = \{(da,db)~|~d\in Z_{+}\}$$

$[(1,1)] = \{(1,1),(2,2),(3,3),...\}$

$[(1,2)] = \{(1,2),(2,4),(3,6),...\}$

$[(2,1)] = \{(2,1),(4,2),(6,3),...\}$

### Example

Define an equivalence relation $\sim$ on $\Z \times \Z$ by $(a,b) \sim (m,n)$ when $a^{2}+b^{2}=m^{2}+n^{2}$. Sjow that this is an equivalence relation and draw the equivalence classes of (1,0), (0,0), (1,1), (1,2) (2,0), and (5,0) alongwith the familiar geometric object for each class.

**Reflexive:** Let $(a,b) \in \Z \times \Z$. Because $a^{2}+b^{2}=a^{2}+b^{2}$ we get $(a,b) \sim (a,b)$

**Symmetric:** Check notes.

**Transitive:** Check notes.

### Partially-ordered Sets, or Posets

A partially ordered set is a set $P$ along with a relation which is usually denoted with $\le$ satisfying the following:

Reflexive: For all $a \in P$, $a \le a$.

AntiSymmetric: For all $a,b \in P$ if $a \le b$ and $b\le a$, then $a=b.$

Transitive: For all $a,b,c \in P$ if $a \le b$ and $b \le c$ then $a\le c$

#### Example

$\Z$ along with the relation $\le$ with its usual meaning is a poset. In fact, for every $a,b \in \Z$, $a\le b$ or $b \le a$. In other words, all pairs of elements of $\Z$ are comparable under $\le$. For this reason, $\Z$ along with $\le$ is called a totally ordered set.

#### Example

Let $n$ be a positive integer and let $D_{n} = \{m \in \Z\ |\ m>0\ and\ m|n\}$ where $m|n$ means m divides n that is n is a multiple of m, that is there is $k \in \Z$ such that $n=mk$.

##### Hasse Diagram of $D_{60}$

![alt text](image-11.png)

#### Example

Let $A$ be any set. Then $\wp(A)$ under the relation $\subseteq$ is a poset.

Reflexive: For any $B \in \wp(A)$, $B \subseteq B$ by definition of subset.

Antisymmetric: For any $B,C \in \wp(A)$ with $B \subseteq C$ and $C \subseteq B$

Transitive: ...

#### Example

Let $X$ be any set. Recall that a partition of $X$ is a set $\{X_1, X_2, ..., X_b\}$ such that

1. $X = X_1 \cup X_2 \cup .... X_b$
2. For each $i$, $X_i \ne \phi$.
3. For all $i\ne j$, $X_i \cap X_j = \phi$

The subsets of $X_i$ of the partition are called blocks. Let $\pi(X)$ the set of all partitions of $X$. Say that $\{X_1, ...., X_q\} \le \{B_1,..., B_t\}$ when foreach $X_i$ there is $B_j$ such that $X_i \subseteq B_j$. When $\{X_1, ...., X_s\} \le \{B_1,..., B_t\}$ we say that $\{X_1, ...., X_q\}$ is a **refinement** ordering of $\{B_1,..., B_t\}$. This refinement relation on $\pi(X)$ is a partially ordered set.

Proving that refinement is a partial order set on $\pi(X)$.

**Reflexive:** Let $\{A_1,...,A_s\} \in \pi(X)$. Because each $A_i \subseteq A_i$, $\{A_1,...,A_i\} \le \{A_1,...,A_i\}$

**Antisymmetry:** Let $\{A_1,...,A_s\}, \{B_1,...,B_t\} \in \pi(X)$. Assume that $\{A_1,...,A_s\}\le \{B_1,...,B_t\} $ and $\{B_1,...,B_t\} \le \{A_1,...,A_s\}$. We'll show that each $i$, $A_i = B_j$ for some $j$. In other words, sshow that $\{A_1,...,A_s\} = \{B_1,...,B_i\} $ that is, each $A_i \in \{B_1,...,B_t\}$ and each $B_j \in \{A_1,..., A_s\}$. By symmetry, we only need to show each $A_i \in \{B_1,...,B_t\}$. Because $\{X_1, ...., X_s\} \le \{B_1,..., B_t\}$, there is some $B_j$ such that $A_i \subseteq B_j$. Because $\{B_1,...,B_i\} \le \{A_1,...,A_s\}$, there is some $k$ such that $A_i \subseteq B_j \subseteq A_k$. This implies that $A_i \subseteq A_k$. Because the partition blocks are disjoint, $A_i \ne \phi$ and $A_i \cap A_k = \phi$ if $i\ne k$, it must be that $A_i = A_k$. Therefore $$A_i \subseteq B_j \subseteq A_i$$
that is, $A_i = B_j$

**Transitivity:** Let $\{A_1,...,A_s\}, \{B_1,...,B_t\}, \{C_1,...,C_u\} \in \pi(X)$. Assume $\{A_1,...,A_s\}\le \{B_1,...,B_t\} $ and $\{B_1,...,B_t\} \le \{C_1,...,C_u\}$. Consider some block $A_i$. Because $\{A_1,...,A_s\}\le \{B_1,...,B_t\} $ there is $B_j$ such that $A_i \subseteq B_j$. Because $\{B_1,...,B_t\} \le \{C_1,...,C_u\}$ there is $C_k$ such that $B_j \subseteq C_k$. Therefore, $A_i \subseteq C_k$. Thus $\{A_1,...,A_s\}\le \{C_1,...,C_u\}$.

#### Example

Let $A$ under the relation $\le_a$ and $B$ under relation $\le_b$ be partially ordered sets. Define a relation $\le$ on $A \times B$ by$$(a_1,b_1) \le (a_2,b_2)\ when\ a_1\le_a a_2\ and\ b_1 \le_b\ b_2$$

prove that $\le$ is a partial order on $A \times B$.

Reflexive: Let $(a,b)\in A\times B$. Because $\le_a$ and $\le_b$ are reflexive, ......, $(a,b) \le(a,b)$

**Antisymmetric:**

**Transitivity:**

$$\rule{6cm}{0.1pt}$$

When $\le$, $\subseteq$, etc (symbol with option for equality) is a partial ordering on a set $P$. Then $\lt$ or $\subset$ have the meaning $a \lt b$ when $a\le b$ and $a \ne b$.

### Example

Let $\le_a$ be a partial ordering on set $A$. Let $\le_b$ be a partial ordering on set $B$. Define $\le$ on $A \times B$ by $$(a_1,b_1)\lt (a_2,b_2)\ when\ either\newline a_1 \le_a a_2~AND~b_1 \le_b b_2\ \newline OR\newline\ a_1 = a_2~AND~b_1 = b_2$$
This is a partial ordering on $A\times B$. Let's prove it.

Reflexive: Let $(a,b)\in A \times B$. Certainly, $a=a$ and $b=b$ thus $(a,b)\le (a,b)$ by the definition of $\le$.

Antisymmetric: Let $(a_1,b_1), (a_2,b_2) \in  A \times B$ such that $(a_1,b_1)\lt (a_2,b_2)$ and $(a_2,b_2)\lt (a_1,b_1)$. By the definition of $\le$, we have $a_1 = a_2$ and $b_1 = b_2$ and $a_2 = a_1$ and $b_2 = b_1$ as the only possible outcome out of 4 outcomes. Thus, $(a_1,b_1) = (a_2,b_2).$

Transitivity: Let $(a_1,b_1), (a_2,b_2), (a_3, b_3) \in  A \times B$. Assume that $(a_1,b_1) \le (a_2,b_2)$ and $(a_2,b_2) \le (a_3, b_3)$.

Possibilities:

1. $a_1 = a_2$ and $a_2 = a_3$ and $b_1 = b_2$ and $b_2 = b_3$
2. $a_1 < a_2$ and $a_2 < a_3$ and $b_1 < b_2$ and $b_2 < b_3$

...

In case 1: $a_1 = a_3\ and\ b_1 = b_3$ thus $(a_1, b_1)\le (a_3, b_3)$
In cases 2,3,4: $a_1 <_a a_3$ and $b_1 <_b b_3$ so $(a_1, b_1)\le (a_3, b_3)$.

## Mathematical Induction

Let $D$ be some set of consecutive integers with a smallest member. E.g. $ D = \{1,2,3,4,...\}$

Mathematical induction is used to prove statements of the type $(\forall n)P(n)$ is true over $D$.

### Simple Induction

**First principle of math. induction.** In order to prove that $(\forall n)P(n)$ is true over $D=\{1,2,3,4,...\}$, it sufficies to prove that:

1. $P(1)$ is true (Base case) and
2. $(\forall n)(P(n) \implies P(n+1)) $ is true (Inductive step)

Why does this prove it's true?

$P(1)$ is true, $P(1) \implies P(2)$ is true therefore $P(2)$ MUST be true.

### Example

Prove that $1+2+3+...+n = \frac{n(n+1)}{2}$ is true for all $n \ge 1$.

In this case, $P(n) = "~1+2+3+....+n=\frac{n(n+1)}{2}\ "$

1. **Base Case (n=1):** $P(1) = 1$ and $P(1) = \frac{1(1+1)}{2} = 1$.

2. **Inductive step:**

Induction Hypo: Assume $P(n)$ is true for some $n\ge 1$.

Target Conclusion: Show that $1 + 2 + ... + n + (n + 1) = \frac{(n+1)(n+2)}{2}$

$=_{by~induction~hypothesis}$

$$\frac{n(n+1)+2(n+1)}{2} = \frac{(n+1)(n+2)}{2}$$
$$n(n+1)+2(n+1) = (n+1)(n+2)$$
$$n^2 + n + 2n + 2 = n^2 + 2n + n + 2$$

### Example

Prove that $1+3+5+...+(2n-1)=n^2$ for all $n\ge1$.

$P(n) = "~1 + 3 + 5 + ... + (2n-1) = n^2~"$

1. **Base Case (n=1):** When $n=1$, $P(1) = 1$ and $1 = 1^2$
2. **Inductive step $(P(n) \implies P(n+1))$:**

Induction Hypo:

Assume that $1 + 3 + 5 + ... + (2n-1) = n^2$ for some $n\ge 1$.

Target Conclusion: Show that $1 + 3 + 5 + ... + (2n-1) + (2n+1) = (n+1)^2$ is also true.

We know $1 + 3 + 5 + ... + (2n-1) + (2n+1) =_{by~induction~hypothesis} n^2 + (2n+1)$ which is equal to $(n+1)^2~\blacksquare$

### Inequalities

If $A= B\le C \le ... \le H$, then $A \le H$

If $A= B\le C < ... \le H$, then $A < H$ (One less than ruins the chain)

If $a \le b$ and $c>0$, then $ca \le cb$

If $a < b$ and $c>0$, then $ca < cb$

If $a < b$ and $c<0$, then $ca > cb$

If $a\le b$ and $c\le d$, then $a+c \le b+d$

If $a< b$ and $c< d$, then $a+c < b+d$

### Example

Prove that $n^2 > 3n+2$ for all $n\ge 4$.

$P(n) = "n^2 > 3n+2"$

1. **Base case (n=4):** When $n=4,n^2 = 4,~and~3n+2=14, ~and~ 16>14$
2. **Induction step**

Assume that $n^2 > 3n+2$ for some $n\ge 4$.

Show that $(n+1)^2 > 3(n+1)+2$ is true.

$(n+1)^2 = n^2 + 2n + 1 >\_{by~induction~hypothesis}~3n+2 + 2n + 1 \ge_{because\ n\ge 4}~3n + 11 > 3n + 5\ \blacksquare$

## Metric Spaces

... See notes ...

### Examples of Metric Spaces

1. $\R$ with $d(x,y)=|x-y|$ is a metric space.

2. $M = \R \times \R$ with $d((x_1,y_1),(x_2,y_2)) = \sqrt{(x_1-x_2)^2+(y_1-y_2)^2}$ is a metric space. (Euclidean Metric)
